src/Primitive/Boolean/VstEnc.v
@@ -1,7 +1,7 @@
 Require Import Core.Core Core.StructNormalizer VstLib VstCallback
         Boolean.Exec ErrorWithWriter DWT.Vst.
 Require Import VST.floyd.proofauto Psatz.
-Require Import Clight.asn_application Clight.BOOLEAN.
+Require Import (* Clight.asn_application *) Clight.BOOLEAN.
 
 Require Import Core.Notations. 
 
@@ -18,34 +18,29 @@ Open Scope Z.
 
 Section Boolean_der_encode_primitive.
 
-Definition cb := _overrun_encoder_cb.
-
-Definition bool_of_int (i : int) := 
-  if (i == 0)%int then false else true.
-
 Definition bool_der_encode_spec : ident * funspec :=
   DECLARE _BOOLEAN_encode_der
-    WITH gv : globals,
-         (* parameters : *)
+    WITH (* parameters : *)
          res: val,  sptr_p : val, sptr_val : int, 
          td_p : val, td : TYPE_descriptor,
          tag_mode : Z, tag : Z,
          (* callback pointer *)
-         (*cb_p : val, *) 
+         cb_p : val, 
          (* callback argument pointer *)                    
          app_key_p : val, app_key_val : val
     PRE [tptr enc_rval_s, tptr type_descriptor_s, tptr tvoid, tint, 
          tuint, tptr cb_type, tptr tvoid]
       PROP (decoder_type td = BOOLEAN_t) (* an implicit contract *)
       PARAMS (res; td_p; sptr_p; Vint (Int.repr tag_mode);
-             Vint (Int.repr tag); gv cb; app_key_p)
-      GLOBALS (gv)
+             Vint (Int.repr tag); cb_p; app_key_p)
+      GLOBALS ()
       SEP (data_at_ Tsh enc_rval_s res;
            data_at_ Tsh type_descriptor_s td_p; 
            data_at Tsh tint (Vint sptr_val) sptr_p;
            data_at_ Tsh tvoid app_key_p;
-           valid_pointer (gv cb);
-           func_ptr callback (gv cb))
+           valid_pointer cb_p;
+           
+           func_ptr' callback cb_p)
     POST [tvoid]
       PROP ()
       LOCAL ()
@@ -57,28 +52,27 @@ Definition bool_der_encode_spec : ident * funspec :=
            data_at Tsh enc_rval_s res_val res;
            data_at_ Tsh type_descriptor_s td_p ; 
            data_at Tsh tint (Vint sptr_val) sptr_p ;
-           data_at_ Tsh tvoid app_key_p ; valid_pointer (gv cb); 
-           func_ptr callback (gv cb); func_ptr' callback (gv cb)).
+           data_at_ Tsh tvoid app_key_p ; valid_pointer cb_p; 
+           func_ptr' callback cb_p).
 
 Definition Gprog := ltac:(with_library prog [der_write_tags_spec; callback_spec;
                                                bool_der_encode_spec]).
 
-Definition if_post1 (gv : globals) cb sptr_p res bool_p erval_p td_p tag_mode 
+Definition if_post1 cb_p sptr_p res bool_p erval_p td_p tag_mode 
            tag app_key_p td sptr_val cb_spec := 
-  PROP(is_pointer_or_null (gv cb))
-  LOCAL(gvars gv;
-        temp _t'6 (Vint (Int.repr 2)); 
+  PROP(is_pointer_or_null (cb_p))
+  LOCAL(temp _t'6 (Vint (Int.repr 2)); 
         temp _t'1 (Vint (Int.repr (encoded {| encoded := 2 |}))); 
         temp _st sptr_p; lvar _bool_value tuchar bool_p;
         lvar _erval (Tstruct _asn_enc_rval_s noattr) erval_p; 
         temp __res res; temp _td td_p; temp _sptr sptr_p; 
         temp _tag_mode (Vint (Int.repr tag_mode)); 
         temp _tag (Vint (Int.repr tag)); 
-        temp _cb (gv cb); temp _app_key app_key_p) 
+        temp _cb (cb_p); temp _app_key app_key_p) 
   SEP(data_at_ Tsh type_descriptor_s td_p; 
       data_at_ Tsh enc_rval_s res; data_at_ Tsh tvoid app_key_p; 
-      func_ptr cb_spec (gv cb); func_ptr' cb_spec (gv cb); 
-      (match (gv cb) with
+      func_ptr' cb_spec (cb_p); 
+      (match (cb_p) with
        | Vint _ => data_at_ Tsh tuchar bool_p
        | _ => data_at Tsh tuchar 
                      (Vubyte (match execErrW (bool_encoder td (bool_of_int sptr_val)) [] with 
@@ -93,22 +87,23 @@ Definition if_post1 (gv : globals) cb sptr_p res bool_p erval_p td_p tag_mode
       field_at Tsh (Tstruct _asn_enc_rval_s noattr) (DOT _structure_ptr) 
                (default_val (tptr tvoid)) erval_p; 
       data_at Tsh tint (Vint sptr_val) sptr_p; 
-      valid_pointer (gv cb)).
+      valid_pointer (cb_p)).
 
-Definition if_post2 (gv : globals) (sptr_val : int) app_key_p (v_bool_value : val) cb_spec 
-           cb v_bool_value v_erval td_p res sptr_p tag_mode tag := 
+Definition if_post2  (sptr_val : int) app_key_p (v_bool_value : val) cb_spec 
+           cb_p v_bool_value v_erval td_p res sptr_p tag_mode tag := 
   PROP()
-  LOCAL(gvars gv; temp _t'6 (Vint (Int.repr 2));
+  LOCAL( temp _t'6 (Vint (Int.repr 2));
         temp _t'1 (Vint (Int.repr (encoded {| encoded := 2 |}))); 
         temp _st sptr_p; lvar _bool_value tuchar v_bool_value;
         lvar _erval (Tstruct _asn_enc_rval_s noattr) v_erval; 
         temp __res res; temp _td td_p; temp _sptr sptr_p;
         temp _tag_mode (Vint (Int.repr tag_mode)); 
         temp _tag (Vint (Int.repr tag)); 
-        temp _cb (gv cb); temp _app_key app_key_p;
+        temp _cb (cb_p); temp _app_key app_key_p;
         temp _t'2 (Vint (Int.repr (if (bool_of_int sptr_val) then 255 else 0))))
   SEP(data_at_ Tsh type_descriptor_s td_p;
-      data_at_ Tsh tvoid app_key_p; func_ptr cb_spec (gv cb);
+      data_at_ Tsh tvoid app_key_p; 
+      func_ptr' cb_spec (cb_p);
       data_at_ Tsh tuchar v_bool_value;
       field_at Tsh (Tstruct _asn_enc_rval_s noattr) (DOT _encoded) 
                (Vint (Int.repr 2)) v_erval;
@@ -118,23 +113,22 @@ Definition if_post2 (gv : globals) (sptr_val : int) app_key_p (v_bool_value : va
       field_at Tsh (Tstruct _asn_enc_rval_s noattr) (DOT _structure_ptr) 
                (default_val (tptr tvoid)) v_erval; 
       data_at_ Tsh enc_rval_s res;
-      data_at Tsh tint (Vint sptr_val) sptr_p; valid_pointer (gv cb)).
+      data_at Tsh tint (Vint sptr_val) sptr_p; valid_pointer (cb_p)).
 
-Definition loop_inv (gv : globals) sptr_p v_bool_value v_erval res td_p tag_mode 
-           tag cb app_key_p (cb_spec : funspec) sptr_val :=
+Definition loop_inv sptr_p v_bool_value v_erval res td_p tag_mode 
+           tag cb_p app_key_p (cb_spec : funspec) sptr_val :=
   PROP()
-  LOCAL(gvars gv; temp _t'4 (Vint (Int.repr 2)); 
+  LOCAL(temp _t'4 (Vint (Int.repr 2)); 
         temp _t'6 (Vint (Int.repr 2)); temp _t'1 (Vint (Int.repr 2)); 
         temp _st sptr_p; lvar _bool_value tuchar v_bool_value;
         lvar _erval (Tstruct _asn_enc_rval_s noattr) v_erval;
         temp __res res; temp _td td_p; temp _sptr sptr_p;
         temp _tag_mode (Vint (Int.repr tag_mode));
-        temp _tag (Vint (Int.repr tag)); temp _cb (gv cb);
+        temp _tag (Vint (Int.repr tag)); temp _cb (cb_p);
         temp _app_key app_key_p)
   SEP(data_at_ Tsh type_descriptor_s td_p;
       data_at_ Tsh enc_rval_s res; data_at_ Tsh tvoid app_key_p;
-      func_ptr callback (gv cb);
-func_ptr' callback (gv cb);
+      func_ptr' callback (cb_p);
       data_at Tsh tuchar (Vubyte (byte_of_bool (bool_of_int sptr_val))) v_bool_value;
       field_at Tsh (Tstruct _asn_enc_rval_s noattr) (DOT _encoded) 
                (Vint (Int.add (Int.repr 2) (Int.repr 1))) v_erval;
@@ -144,7 +138,7 @@ func_ptr' callback (gv cb);
       field_at Tsh (Tstruct _asn_enc_rval_s noattr) (DOT _structure_ptr)
                (default_val (tptr tvoid)) v_erval;
       data_at Tsh tint (Vint sptr_val) sptr_p;
-      valid_pointer (gv cb)).
+      valid_pointer (cb_p)).
 
 Theorem bool_der_encode : semax_body Vprog Gprog 
                                      (normalize_function f_BOOLEAN_encode_der
@@ -153,18 +147,18 @@ Theorem bool_der_encode : semax_body Vprog Gprog
 Proof.
   start_function; rename H into DT.
   forward.
-  forward_call (td_p, td, 1, tag_mode, 0, tag, (gv cb), app_key_p, app_key_val).
+  forward_call (td_p, td, 1, tag_mode, 0, tag, cb_p, app_key_p, app_key_val).
   rewrite Exec.eval_dwt_boolean by assumption.
   unfold_data_at_ v_erval; unfold_data_at (data_at _ _ _ v_erval).
   forward.
   forward.
   forward_if; [contradiction|clear H].
-  forward_if (if_post1 gv cb sptr_p res v_bool_value v_erval td_p tag_mode tag 
+  forward_if (if_post1 cb_p sptr_p res v_bool_value v_erval td_p tag_mode tag 
                        app_key_p td sptr_val callback); unfold if_post1.
   * (* if(cb) = true *)
     forward.
     (* bool_value = *st ? 0xff : 0; /* 0xff mandated by DER */ *)
-    forward_if (if_post2 gv sptr_val app_key_p v_bool_value callback cb v_bool_value 
+    forward_if (if_post2 sptr_val app_key_p v_bool_value callback cb_p v_bool_value 
                          v_erval td_p res sptr_p tag_mode tag); unfold if_post2.
     - (* if(b) = true *)
       forward; unfold if_post2; entailer!.
@@ -174,13 +168,14 @@ Proof.
     - (* if(b) = false *)
       forward; unfold if_post2; entailer!.
     - forward.
-      make_func_ptr cb.
-      forward_call ([sptr_val], v_bool_value, 1, app_key_p).
+      forward_call 
+             ([(Int.zero_ext 8 (Int.repr (if bool_of_int sptr_val then 255 else 0)))],
+              v_bool_value, 1, app_key_p).                                                 
       forward_if; [congruence|].
       ** (* cb() >= 0 *)
         unfold if_post1; forward.
          entailer!.
-         destruct (gv cb); intuition.
+         destruct (cb_p); intuition.
          rewrite exec_boolean_enc by assumption.
          unfold bool_of_int.
          destruct (sptr_val == 0)%int eqn : S; entailer!.
@@ -193,10 +188,10 @@ Proof.
     forward.
     forward.
     unfold construct_enc_rval, encoded, last.
-    forward_loop (loop_inv gv sptr_p v_bool_value v_erval res td_p tag_mode tag
-                                cb app_key_p callback sptr_val); unfold loop_inv.
+    forward_loop (loop_inv sptr_p v_bool_value v_erval res td_p tag_mode tag
+                                cb_p app_key_p callback sptr_val); unfold loop_inv.
     - entailer!.
-      destruct (gv cb); intuition.
+      destruct cb_p; intuition.
     - 
       unfold_data_at_ res; unfold_data_at (data_at _ _ _ res).
       repeat forward.
